Interop stub: Add support for ghost arguments

src/arch/x64/interop/Main.ml
@@ -7,10 +7,13 @@ open Interop_Printer
 let gcmencrypt = ("gcmencrypt", [
   ("plain_b", TBuffer TUInt128); ("plain_num_bytes", TBase TUInt64);
   ("auth_b", TBuffer TUInt128); ("auth_num_bytes", TBase TUInt64);
-  ("iv_b", TBuffer TUInt128); ("keys_b", TBuffer TUInt128);
+  ("iv_b", TBuffer TUInt128); 
+  ("key", TGhost "aes_key_LE AES_128"); ("keys_b", TBuffer TUInt128);
   ("cipher_b", TBuffer TUInt128); ("tag_b", TBuffer TUInt128)
   ])
 
-let _ = print_string (translate_vale Linux X86 gcmencrypt)
+let os = Windows 
+
+let _ = print_string (translate_vale os X86 gcmencrypt)
 let _ = print_newline()
-let _ = print_string (translate_lowstar Linux X86 gcmencrypt)
+let _ = print_string (translate_lowstar os X86 gcmencrypt)
