src/arch/x64/interop/GCMEncrypt.fst
@@ -14,6 +14,7 @@ open X64.Machine_s
 open X64.Memory_i_s
 open X64.Vale.State_i
 open X64.Vale.Decls_i
+open AES_s
 #set-options "--z3rlimit 40"
 
 open Vale_gcmencrypt
@@ -39,8 +40,8 @@ unfold
 let locs_disjoint (ls:list b8) : Type0 = normalize (locs_disjoint_rec ls)
 
 // TODO: Complete with your pre- and post-conditions
-let pre_cond (h:HS.mem) (plain_b:b8) (plain_num_bytes:nat64) (auth_b:b8) (auth_num_bytes:nat64) (iv_b:b8) (keys_b:b8) (cipher_b:b8) (tag_b:b8) = live h plain_b /\ live h auth_b /\ live h iv_b /\ live h keys_b /\ live h cipher_b /\ live h tag_b /\ locs_disjoint [plain_b;auth_b;iv_b;keys_b;cipher_b;tag_b] /\ length plain_b % 16 == 0 /\ length auth_b % 16 == 0 /\ length iv_b % 16 == 0 /\ length keys_b % 16 == 0 /\ length cipher_b % 16 == 0 /\ length tag_b % 16 == 0
-let post_cond (h0:HS.mem) (h1:HS.mem) (plain_b:b8) (plain_num_bytes:nat64) (auth_b:b8) (auth_num_bytes:nat64) (iv_b:b8) (keys_b:b8) (cipher_b:b8) (tag_b:b8) = live h0 plain_b /\ live h0 auth_b /\ live h0 iv_b /\ live h0 keys_b /\ live h0 cipher_b /\ live h0 tag_b /\ live h1 plain_b /\ live h1 auth_b /\ live h1 iv_b /\ live h1 keys_b /\ live h1 cipher_b /\ live h1 tag_b /\ length plain_b % 16 == 0 /\ length auth_b % 16 == 0 /\ length iv_b % 16 == 0 /\ length keys_b % 16 == 0 /\ length cipher_b % 16 == 0 /\ length tag_b % 16 == 0
+let pre_cond (h:HS.mem) (plain_b:b8) (plain_num_bytes:nat64) (auth_b:b8) (auth_num_bytes:nat64) (iv_b:b8) (key:Ghost.erased (aes_key_LE AES_128)) (keys_b:b8) (cipher_b:b8) (tag_b:b8) = live h plain_b /\ live h auth_b /\ live h iv_b /\ live h keys_b /\ live h cipher_b /\ live h tag_b /\ locs_disjoint [plain_b;auth_b;iv_b;keys_b;cipher_b;tag_b] /\ length plain_b % 16 == 0 /\ length auth_b % 16 == 0 /\ length iv_b % 16 == 0 /\ length keys_b % 16 == 0 /\ length cipher_b % 16 == 0 /\ length tag_b % 16 == 0
+let post_cond (h0:HS.mem) (h1:HS.mem) (plain_b:b8) (plain_num_bytes:nat64) (auth_b:b8) (auth_num_bytes:nat64) (iv_b:b8) (key:Ghost.erased (aes_key_LE AES_128)) (keys_b:b8) (cipher_b:b8) (tag_b:b8) = live h0 plain_b /\ live h0 auth_b /\ live h0 iv_b /\ live h0 keys_b /\ live h0 cipher_b /\ live h0 tag_b /\ live h1 plain_b /\ live h1 auth_b /\ live h1 iv_b /\ live h1 keys_b /\ live h1 cipher_b /\ live h1 tag_b /\ length plain_b % 16 == 0 /\ length auth_b % 16 == 0 /\ length iv_b % 16 == 0 /\ length keys_b % 16 == 0 /\ length cipher_b % 16 == 0 /\ length tag_b % 16 == 0
 
 //The initial registers and xmms
 assume val init_regs:reg -> nat64
@@ -48,8 +49,8 @@ assume val init_xmms:xmm -> quad32
 
 #set-options "--initial_fuel 9 --max_fuel 9 --initial_ifuel 2 --max_ifuel 2"
 // TODO: Prove these two lemmas if they are not proven automatically
-let implies_pre (h0:HS.mem) (plain_b:b8) (plain_num_bytes:nat64) (auth_b:b8) (auth_num_bytes:nat64) (iv_b:b8) (keys_b:b8) (cipher_b:b8) (tag_b:b8)  (stack_b:b8) : Lemma
-  (requires pre_cond h0 plain_b plain_num_bytes auth_b auth_num_bytes iv_b keys_b cipher_b tag_b /\ B.length stack_b == 16 /\ live h0 stack_b /\ locs_disjoint [stack_b;plain_b;auth_b;iv_b;keys_b;cipher_b;tag_b])
+let implies_pre (h0:HS.mem) (plain_b:b8) (plain_num_bytes:nat64) (auth_b:b8) (auth_num_bytes:nat64) (iv_b:b8) (key:Ghost.erased (aes_key_LE AES_128)) (keys_b:b8) (cipher_b:b8) (tag_b:b8)  (stack_b:b8) : Lemma
+  (requires pre_cond h0 plain_b plain_num_bytes auth_b auth_num_bytes iv_b key keys_b cipher_b tag_b /\ B.length stack_b == 16 /\ live h0 stack_b /\ locs_disjoint [stack_b;plain_b;auth_b;iv_b;keys_b;cipher_b;tag_b])
   (ensures (
 B.length stack_b == 16 /\ live h0 stack_b /\ locs_disjoint [stack_b;plain_b;auth_b;iv_b;keys_b;cipher_b;tag_b] /\ (  let buffers = stack_b::plain_b::auth_b::iv_b::keys_b::cipher_b::tag_b::[] in
   let (mem:mem) = {addrs = addrs; ptrs = buffers; hs = h0} in
@@ -79,7 +80,7 @@ B.length stack_b == 16 /\ live h0 stack_b /\ locs_disjoint [stack_b;plain_b;auth
   length_t_eq (TBase TUInt128) keys_b;
   length_t_eq (TBase TUInt128) cipher_b;
   length_t_eq (TBase TUInt128) tag_b;
-  va_pre (va_code_gcmencrypt ()) s0 plain_b plain_num_bytes auth_b auth_num_bytes iv_b keys_b cipher_b tag_b ))) =
+  va_pre (va_code_gcmencrypt ()) s0 plain_b plain_num_bytes auth_b auth_num_bytes iv_b (Ghost.reveal key) keys_b cipher_b tag_b ))) =
   length_t_eq (TBase TUInt128) plain_b;
   length_t_eq (TBase TUInt128) auth_b;
   length_t_eq (TBase TUInt128) iv_b;
@@ -88,10 +89,10 @@ B.length stack_b == 16 /\ live h0 stack_b /\ locs_disjoint [stack_b;plain_b;auth
   length_t_eq (TBase TUInt128) tag_b;
   ()
 
-let implies_post (va_s0:va_state) (va_sM:va_state) (va_fM:va_fuel) (plain_b:b8) (plain_num_bytes:nat64) (auth_b:b8) (auth_num_bytes:nat64) (iv_b:b8) (keys_b:b8) (cipher_b:b8) (tag_b:b8)  (stack_b:b8) : Lemma
-  (requires pre_cond va_s0.mem.hs plain_b plain_num_bytes auth_b auth_num_bytes iv_b keys_b cipher_b tag_b /\
-    va_post (va_code_gcmencrypt ()) va_s0 va_sM va_fM plain_b plain_num_bytes auth_b auth_num_bytes iv_b keys_b cipher_b tag_b )
-  (ensures post_cond va_s0.mem.hs va_sM.mem.hs plain_b plain_num_bytes auth_b auth_num_bytes iv_b keys_b cipher_b tag_b ) =
+let implies_post (va_s0:va_state) (va_sM:va_state) (va_fM:va_fuel) (plain_b:b8) (plain_num_bytes:nat64) (auth_b:b8) (auth_num_bytes:nat64) (iv_b:b8) (key:Ghost.erased (aes_key_LE AES_128)) (keys_b:b8) (cipher_b:b8) (tag_b:b8)  (stack_b:b8) : Lemma
+  (requires pre_cond va_s0.mem.hs plain_b plain_num_bytes auth_b auth_num_bytes iv_b key keys_b cipher_b tag_b /\
+    va_post (va_code_gcmencrypt ()) va_s0 va_sM va_fM plain_b plain_num_bytes auth_b auth_num_bytes iv_b (Ghost.reveal key) keys_b cipher_b tag_b )
+  (ensures post_cond va_s0.mem.hs va_sM.mem.hs plain_b plain_num_bytes auth_b auth_num_bytes iv_b key keys_b cipher_b tag_b ) =
   length_t_eq (TBase TUInt128) plain_b;
   length_t_eq (TBase TUInt128) auth_b;
   length_t_eq (TBase TUInt128) iv_b;
@@ -100,13 +101,13 @@ let implies_post (va_s0:va_state) (va_sM:va_state) (va_fM:va_fuel) (plain_b:b8) 
   length_t_eq (TBase TUInt128) tag_b;
   ()
 
-val gcmencrypt: plain_b:b8 -> plain_num_bytes:nat64 -> auth_b:b8 -> auth_num_bytes:nat64 -> iv_b:b8 -> keys_b:b8 -> cipher_b:b8 -> tag_b:b8 -> Stack unit
-	(requires (fun h -> pre_cond h plain_b plain_num_bytes auth_b auth_num_bytes iv_b keys_b cipher_b tag_b ))
-	(ensures (fun h0 _ h1 -> post_cond h0 h1 plain_b plain_num_bytes auth_b auth_num_bytes iv_b keys_b cipher_b tag_b ))
+val gcmencrypt: plain_b:b8 -> plain_num_bytes:nat64 -> auth_b:b8 -> auth_num_bytes:nat64 -> iv_b:b8 -> key:Ghost.erased (aes_key_LE AES_128) -> keys_b:b8 -> cipher_b:b8 -> tag_b:b8 -> Stack unit
+	(requires (fun h -> pre_cond h plain_b plain_num_bytes auth_b auth_num_bytes iv_b key keys_b cipher_b tag_b ))
+	(ensures (fun h0 _ h1 -> post_cond h0 h1 plain_b plain_num_bytes auth_b auth_num_bytes iv_b key keys_b cipher_b tag_b ))
 
-val ghost_gcmencrypt: plain_b:b8 -> plain_num_bytes:nat64 -> auth_b:b8 -> auth_num_bytes:nat64 -> iv_b:b8 -> keys_b:b8 -> cipher_b:b8 -> tag_b:b8 ->  stack_b:b8 -> (h0:HS.mem{pre_cond h0 plain_b plain_num_bytes auth_b auth_num_bytes iv_b keys_b cipher_b tag_b /\ B.length stack_b == 16 /\ live h0 stack_b /\ locs_disjoint [stack_b;plain_b;auth_b;iv_b;keys_b;cipher_b;tag_b]}) -> GTot (h1:HS.mem{post_cond h0 h1 plain_b plain_num_bytes auth_b auth_num_bytes iv_b keys_b cipher_b tag_b })
+val ghost_gcmencrypt: plain_b:b8 -> plain_num_bytes:nat64 -> auth_b:b8 -> auth_num_bytes:nat64 -> iv_b:b8 -> key:Ghost.erased (aes_key_LE AES_128) -> keys_b:b8 -> cipher_b:b8 -> tag_b:b8 ->  stack_b:b8 -> (h0:HS.mem{pre_cond h0 plain_b plain_num_bytes auth_b auth_num_bytes iv_b key keys_b cipher_b tag_b /\ B.length stack_b == 16 /\ live h0 stack_b /\ locs_disjoint [stack_b;plain_b;auth_b;iv_b;keys_b;cipher_b;tag_b]}) -> GTot (h1:HS.mem{post_cond h0 h1 plain_b plain_num_bytes auth_b auth_num_bytes iv_b key keys_b cipher_b tag_b })
 
-let ghost_gcmencrypt plain_b plain_num_bytes auth_b auth_num_bytes iv_b keys_b cipher_b tag_b stack_b h0 =
+let ghost_gcmencrypt plain_b plain_num_bytes auth_b auth_num_bytes iv_b key keys_b cipher_b tag_b stack_b h0 =
   let buffers = stack_b::plain_b::auth_b::iv_b::keys_b::cipher_b::tag_b::[] in
   let (mem:mem) = {addrs = addrs; ptrs = buffers; hs = h0} in
   let addr_plain_b = addrs plain_b in
@@ -135,8 +136,8 @@ let ghost_gcmencrypt plain_b plain_num_bytes auth_b auth_num_bytes iv_b keys_b c
   length_t_eq (TBase TUInt128) keys_b;
   length_t_eq (TBase TUInt128) cipher_b;
   length_t_eq (TBase TUInt128) tag_b;
-  implies_pre h0 plain_b plain_num_bytes auth_b auth_num_bytes iv_b keys_b cipher_b tag_b stack_b ;
-  let s1, f1 = va_lemma_gcmencrypt (va_code_gcmencrypt ()) s0 plain_b plain_num_bytes auth_b auth_num_bytes iv_b keys_b cipher_b tag_b  in
+  implies_pre h0 plain_b plain_num_bytes auth_b auth_num_bytes iv_b key keys_b cipher_b tag_b stack_b ;
+  let s1, f1 = va_lemma_gcmencrypt (va_code_gcmencrypt ()) s0 plain_b plain_num_bytes auth_b auth_num_bytes iv_b (Ghost.reveal key) keys_b cipher_b tag_b  in
   // Ensures that the Vale execution was correct
   assert(s1.ok);
   // Ensures that the callee_saved registers are correct
@@ -148,12 +149,12 @@ let ghost_gcmencrypt plain_b plain_num_bytes auth_b auth_num_bytes iv_b keys_b c
   assert(s0.regs R15 == s1.regs R15);
   // Ensures that va_code_gcmencrypt is actually Vale code, and that s1 is the result of executing this code
   assert (va_ensure_total (va_code_gcmencrypt ()) s0 s1 f1);
-  implies_post s0 s1 f1 plain_b plain_num_bytes auth_b auth_num_bytes iv_b keys_b cipher_b tag_b stack_b ;
+  implies_post s0 s1 f1 plain_b plain_num_bytes auth_b auth_num_bytes iv_b key keys_b cipher_b tag_b stack_b ;
   s1.mem.hs
 
-let gcmencrypt plain_b plain_num_bytes auth_b auth_num_bytes iv_b keys_b cipher_b tag_b  =
+let gcmencrypt plain_b plain_num_bytes auth_b auth_num_bytes iv_b key keys_b cipher_b tag_b  =
   push_frame();
   let (stack_b:b8) = B.alloca (UInt8.uint_to_t 0) (UInt32.uint_to_t 16) in
   let h0 = get() in
-  st_put h0 (fun h -> pre_cond h plain_b plain_num_bytes auth_b auth_num_bytes iv_b keys_b cipher_b tag_b /\ B.length stack_b == 16 /\ live h stack_b /\ locs_disjoint [stack_b;plain_b;auth_b;iv_b;keys_b;cipher_b;tag_b]) (ghost_gcmencrypt plain_b plain_num_bytes auth_b auth_num_bytes iv_b keys_b cipher_b tag_b stack_b);
+  st_put h0 (fun h -> pre_cond h plain_b plain_num_bytes auth_b auth_num_bytes iv_b key keys_b cipher_b tag_b /\ B.length stack_b == 16 /\ live h stack_b /\ locs_disjoint [stack_b;plain_b;auth_b;iv_b;keys_b;cipher_b;tag_b]) (ghost_gcmencrypt plain_b plain_num_bytes auth_b auth_num_bytes iv_b key keys_b cipher_b tag_b stack_b);
   pop_frame()
